I've modified the UART example to show how 32-bit memory mapped registers can be modelled (in response to an email from Jianjun Duan).

examples/ARM/experimental/lpc_uartScript.sml
@@ -10,14 +10,14 @@ val _ = new_theory "lpc_uart";
 (* We define the state of a UART interface *)
 
 val _ = Hol_datatype `
-  uart0_state = <| 
+  uart0_state = <|
 
     (* physical state components *)
 
-    U0RBR : word8;  (* receive buffer *)
-    U0THR : word8;  (* transmit holding buffer *)
-    U0LCR : word8;  (* line control register *)
-    U0LSR : word8;  (* line status register *)
+    U0RBR : word8;   (* receive buffer *)
+    U0THR : word8;   (* transmit holding buffer *)
+    U0LCR : word32;  (* line control register *)
+    U0LSR : word32;  (* line status register *)
 
     (* logical state components *)
 
@@ -43,10 +43,10 @@ val _ = Hol_datatype `
 
 val uart0_ok_def = Define `
   uart0_ok current_time (uart0:uart0_state) =
-    (* U0LCR must be in a usable state *) 
+    (* U0LCR must be in a usable state *)
     (uart0.U0LCR ' 7 = F) /\
     (* U0LSR bit 0 and bit 5 indicate whether U0RBR and U0THR, resp., are ready for use *)
-    (uart0.U0LSR ' 0 = (uart0.input_time <= current_time) /\ ~(uart0.input_list = [])) /\ 
+    (uart0.U0LSR ' 0 = (uart0.input_time <= current_time) /\ ~(uart0.input_list = [])) /\
     (uart0.U0LSR ' 5 = (uart0.output_time <= current_time)) /\
     (* Content of U0RBR and U0THR is determined by state of U0LSR *)
     (?w. uart0.U0RBR = if uart0.U0LSR ' 0 then HD (uart0.input_list) else w) /\
@@ -56,108 +56,189 @@ val uart0_ok_def = Define `
 (* We define what addresses are owned by UART0, and whether they can be read and written *)
 
 val UART0_addresses_def = Define `
-  UART0_addresses = {0xE000C000w;
-                     0xE000C004w;
-                     0xE000C008w;
-                     0xE000C00Cw;
-                     0xE000C014w;  
-                     0xE000C01Cw;
-                     0xE000C020w;
-                     0xE000C028w;  
-                     0xE000C030w} : word32 set`;
+  UART0_addresses =
+    { x | 0xE000C000w <=+ x /\ x <+ 0xE000C034w } : word32 set`;
 
 
 (* We define what value the core sees if it reads one of UART0's addresses *)
 
+val mm_byte_reader_def = Define `
+  mm_byte_reader (a:word32) (b:word8) = (a =+ b)`;
+
+val mm_word_reader_def = Define `
+  mm_word_reader (a:word32) (w:word32) =
+    (a+0w =+ ( 7 ><  0) w) o
+    (a+1w =+ (15 ><  8) w) o
+    (a+2w =+ (23 >< 16) w) o
+    (a+3w =+ (31 >< 24) w)`;
+
 val UART0_read_def = Define `
-  UART0_read (uart0:uart0_state) a = 
-    if a = 0xE000C000w then w2w (uart0.U0RBR) else
-    if a = 0xE000C00Cw then w2w (uart0.U0LCR) else
-    if a = 0xE000C014w then w2w (uart0.U0LSR) else ARB`;
+  UART0_read (uart0:uart0_state) =
+   (mm_byte_reader 0xE000C000w (uart0.U0RBR) o
+    mm_word_reader 0xE000C00Cw (uart0.U0LCR) o
+    mm_word_reader 0xE000C014w (uart0.U0LSR)) (\a. ARB)`;
 
 
 (* We define the possible next states (some s2) after a clock tick (starting from s1) *)
 
-val MEM_WRITE_VALUE_def = Define `
-  (MEM_WRITE_VALUE a [] = ARB) /\
-  (MEM_WRITE_VALUE a ((MEM_READ w)::xs) = MEM_WRITE_VALUE a xs) /\
-  (MEM_WRITE_VALUE a ((MEM_WRITE w v)::xs) = if a = w then v else MEM_WRITE_VALUE a xs)`;
+val BYTE_WRITTEN_TO_MEM_def = Define `
+  (BYTE_WRITTEN_TO_MEM a [] = ARB) /\
+  (BYTE_WRITTEN_TO_MEM a ((MEM_READ w)::xs) = BYTE_WRITTEN_TO_MEM a xs) /\
+  (BYTE_WRITTEN_TO_MEM a ((MEM_WRITE w v)::xs) = if a = w then v else BYTE_WRITTEN_TO_MEM a xs)`;
+
+val _ = wordsLib.guess_lengths();
+val WORD_WRITTEN_TO_MEM_def = Define `
+  WORD_WRITTEN_TO_MEM a accesses =
+    BYTE_WRITTEN_TO_MEM (a+3w) accesses @@
+    BYTE_WRITTEN_TO_MEM (a+2w) accesses @@
+    BYTE_WRITTEN_TO_MEM (a+1w) accesses @@
+    BYTE_WRITTEN_TO_MEM (a+0w) accesses`;
+
+val ADDR_SET_def = Define `
+  (ADDR_SET [] = {}) /\
+  (ADDR_SET ((MEM_READ a)::xs) = a INSERT ADDR_SET xs) /\
+  (ADDR_SET ((MEM_WRITE a b)::xs) = a INSERT ADDR_SET xs)`;
+
+val ALL_OR_NOTHING_def = Define `
+  ALL_OR_NOTHING x a = (x INTER a = a) \/ (x INTER a = {})`;
+
+val IS_MEM_READ_def = Define `
+  (IS_MEM_READ (MEM_READ a) = T) /\ (IS_MEM_READ _ = F)`;
+
+val IS_MEM_WRITE_def = Define `
+  (IS_MEM_WRITE (MEM_WRITE a w) = T) /\ (IS_MEM_WRITE _ = F)`;
+
+(* read-write enabled *)
+val REG32_RW_NEXT_def = Define `
+  REG32_RW_NEXT addr pre_value accesses post_value =
+    let a = {addr; addr+1w; addr+2w; addr+3w} in
+    let reads = ADDR_SET (FILTER IS_MEM_READ accesses) in
+    let writes = ADDR_SET (FILTER IS_MEM_WRITE accesses) in
+      ALL_OR_NOTHING reads a /\
+      ALL_OR_NOTHING writes a /\
+      (post_value = if addr IN writes
+                    then WORD_WRITTEN_TO_MEM addr accesses
+                    else pre_value)`;
+
+
+(* read only version *)
+val REG32_RO_NEXT_def = Define `
+  REG32_RO_NEXT addr accesses =
+    let a = {addr; addr+1w; addr+2w; addr+3w} in
+    let reads = ADDR_SET (FILTER IS_MEM_READ accesses) in
+    let writes = ADDR_SET (FILTER IS_MEM_WRITE accesses) in
+      ALL_OR_NOTHING reads a /\
+      (a INTER writes = {})`;
+
 
 val UART0_NEXT_def = Define `
   UART0_NEXT current_time (accesses:memory_access list) (s1:uart0_state) (s2:uart0_state) =
 
-    (* both before and after state must be consistent, i.e. logical components of 
+    (* both before and after state must be consistent, i.e. logical components of
        each state must agree with physical components of resp. state. *)
     uart0_ok current_time s1 /\ uart0_ok (current_time+1) s2 /\
 
     (* if read happened then ... else ... *)
-    (if MEM (MEM_READ 0xE000C000w) accesses then 
+    (if MEM (MEM_READ 0xE000C000w) accesses then
        (s1.U0LSR ' 0 = T) /\ (* fail if UART0 was not ready for a read *)
        (s2.input_list = TL s1.input_list) (* pop one element off input list *)
        (* implicity let input_delay in s2 be any natural number *)
-     else 
+     else
        (* if no read happened then do nothing *)
-       (s2.input_time = s1.input_time) /\ 
+       (s2.input_time = s1.input_time) /\
        (s2.input_list = s1.input_list)) /\
 
     (* if write happened then ... else ... *)
-    (if ?w. MEM (MEM_WRITE 0xE000C000w w) accesses then 
+    (if ?w. MEM (MEM_WRITE 0xE000C000w w) accesses then
        (s1.U0LSR ' 5 = T) /\ (* fail if UART0 was not ready for a write *)
-       (s2.output_list = w2w (MEM_WRITE_VALUE 0xE000C000w accesses) :: s1.output_list) (* cons new output *)
+       (s2.output_list = w2w (BYTE_WRITTEN_TO_MEM 0xE000C000w accesses) :: s1.output_list) (* cons new output *)
        (* implicity let output_delay in s2 be any natural number *)
-     else 
+     else
        (* if no write happened then do nothing *)
-       (s2.output_time = s1.output_time) /\ 
-       (s2.output_list = s1.output_list))`;
+       (s2.output_time = s1.output_time) /\
+       (s2.output_list = s1.output_list)) /\
+
+    (* the 32-bit memory-mapped registers *)
+    REG32_RW_NEXT 0xE000C00Cw (s1.U0LCR) accesses (s2.U0LCR) /\
+    REG32_RO_NEXT 0xE000C014w accesses`;
 
 
-(* Definition of the public parts of UART0 state *)
+
+
+(* A lemma needed later on *)
+
+val REG32_NEXT_NIL = prove(
+  ``!x w1 w2. (REG32_RW_NEXT x w1 [] w2 = (w1 = w2)) /\
+              (REG32_RO_NEXT x [] = T)``,
+  SIMP_TAC std_ss [REG32_RW_NEXT_def,REG32_RO_NEXT_def,LET_DEF,FILTER,ADDR_SET_def,
+     pred_setTheory.NOT_IN_EMPTY,ALL_OR_NOTHING_def,pred_setTheory.INTER_EMPTY]
+  THEN METIS_TAC []);
+
+val BIT_UPDATE_def = Define `
+  BIT_UPDATE i b (w:'a word) = (FCP j. if i = j then b else w ' j):'a word`;
+
+val APPLY_BIT_UPDATE_THM = store_thm("APPLY_BIT_UPDATE_THM",
+  ``!i j b w.
+      j < dimindex (:'a) ==>
+      (BIT_UPDATE i b (w:'a word) ' j = if i = j then b else w ' j)``,
+  SIMP_TAC std_ss [fcpTheory.CART_EQ,BIT_UPDATE_def,fcpTheory.FCP_BETA]);
+
+val UART0_NEXT_EXISTS = store_thm("UART0_NEXT_EXISTS",
+  ``!t s1. uart0_ok t s1 ==> ?s2. UART0_NEXT t [] s1 s2``,
+  SIMP_TAC std_ss [UART0_NEXT_def,uart0_ok_def,MEM,REG32_NEXT_NIL]
+  THEN REPEAT STRIP_TAC
+  THEN EXISTS_TAC
+  ``<| U0RBR := if s1.input_time <= t + 1 /\ s1.input_list <> [] then HD s1.input_list else ARB;
+       U0THR := if s1.output_time <= t + 1 then ARB else HD s1.output_list;
+       U0LCR := s1.U0LCR;
+       U0LSR := BIT_UPDATE 0 (s1.input_time <= t + 1 /\ s1.input_list <> [])
+               (BIT_UPDATE 5 (s1.output_time <= t + 1) s1.U0LSR);
+       input_list  := s1.input_list;
+       input_time  := s1.input_time;
+       output_list := s1.output_list;
+       output_time := s1.output_time |>``
+  THEN SRW_TAC [] [APPLY_BIT_UPDATE_THM]);
 
 val UART0_READ_def = Define `
   UART0_READ (uart0:uart0_state) =
     (uart0.input_list,uart0.input_time,uart0.output_list,uart0.output_time)`;
 
 
-(* UART0 does nothing observable when left untouched, 
+(* -- old part of script commented out, but might be used in the future
+
+
+
+(* UART0 does nothing observable when left untouched,
    similarly reading LSR has no observable effect. *)
-
-val BIT_UPDATE_def = Define `
-  BIT_UPDATE i b (w:'a word) = (FCP j. if i = j then b else w ' j):'a word`; 
-
-val APPLY_BIT_UPDATE_THM = store_thm("APPLY_BIT_UPDATE_THM",
-  ``!i j b w. 
-      j < dimindex (:'a) ==>
-      (BIT_UPDATE i b (w:'a word) ' j = if i = j then b else w ' j)``,
-  SIMP_TAC std_ss [fcpTheory.CART_EQ,BIT_UPDATE_def,fcpTheory.FCP_BETA]);
 
 val UART0_NEXT_NIL = store_thm("UART0_NEXT_NIL",
   ``!t s1 s2.
-      UART0_NEXT t [] s1 s2 = 
+      UART0_NEXT t [] s1 s2 =
       uart0_ok t s1 /\ uart0_ok (t+1) s2 /\ (UART0_READ s1 = UART0_READ s2)``,
-  SIMP_TAC std_ss [UART0_READ_def,UART0_NEXT_def,MEM] THEN METIS_TAC []);  
+  SIMP_TAC std_ss [UART0_READ_def,UART0_NEXT_def,MEM] THEN METIS_TAC []);
 
 val UART0_NEXT_READ_LSR = store_thm("UART0_NEXT_READ_LSR",
   ``!t s1 s2.
-      UART0_NEXT t [MEM_READ 0xE000C014w] s1 s2 = 
+      UART0_NEXT t [MEM_READ 0xE000C014w] s1 s2 =
       uart0_ok t s1 /\ uart0_ok (t+1) s2 /\ (UART0_READ s1 = UART0_READ s2)``,
   SIMP_TAC (std_ss++SIZES_ss) [UART0_READ_def,UART0_NEXT_def,MEM,
-    memory_access_11,memory_access_distinct,n2w_11] THEN METIS_TAC []);  
+    memory_access_11,memory_access_distinct,n2w_11] THEN METIS_TAC []);
 
 val UART0_NEXT_EXISTS = store_thm("UART0_NEXT_EXISTS",
-  ``!t s1. uart0_ok t s1 ==> 
-           ?s2. UART0_NEXT t [] s1 s2 /\ 
+  ``!t s1. uart0_ok t s1 ==>
+           ?s2. UART0_NEXT t [] s1 s2 /\
                 UART0_NEXT t [MEM_READ 0xE000C014w] s1 s2``,
   SIMP_TAC std_ss [UART0_NEXT_NIL,UART0_NEXT_READ_LSR,uart0_ok_def]
   THEN REPEAT STRIP_TAC
-  THEN EXISTS_TAC 
+  THEN EXISTS_TAC
   ``<| U0RBR := if s1.input_time <= t + 1 /\ s1.input_list <> [] then HD s1.input_list else ARB;
        U0THR := if s1.output_time <= t + 1 then ARB else HD s1.output_list;
        U0LCR := s1.U0LCR;
-       U0LSR := BIT_UPDATE 0 (s1.input_time <= t + 1 /\ s1.input_list <> []) 
+       U0LSR := BIT_UPDATE 0 (s1.input_time <= t + 1 /\ s1.input_list <> [])
                (BIT_UPDATE 5 (s1.output_time <= t + 1) s1.U0LSR);
-       input_list  := s1.input_list;  
-       input_time  := s1.input_time;         
-       output_list := s1.output_list;  
+       input_list  := s1.input_list;
+       input_time  := s1.input_time;
+       output_list := s1.output_list;
        output_time := s1.output_time |>``
   THEN SRW_TAC [] [UART0_READ_def,APPLY_BIT_UPDATE_THM]);
 
@@ -168,17 +249,17 @@ val UART0_READ = store_thm("UART0_READ",
   ``!t s1 w. uart0_ok t s1 /\ s1.U0LSR ' 0 ==>
              ?s2. UART0_NEXT t [MEM_READ 0xE000C000w] s1 s2``,
   SIMP_TAC std_ss [uart0_ok_def,UART0_NEXT_def,MEM,memory_access_11,
-    memory_access_distinct,MEM_WRITE_VALUE_def]
+    memory_access_distinct,BYTE_WRITTEN_TO_MEM_def]
   THEN REPEAT STRIP_TAC
-  THEN EXISTS_TAC 
+  THEN EXISTS_TAC
   ``<| U0RBR := ARB;
        U0THR := if s1.output_time <= t + 1 then ARB else HD s1.output_list;
        U0LCR := s1.U0LCR;
-       U0LSR := BIT_UPDATE 0 F 
+       U0LSR := BIT_UPDATE 0 F
                (BIT_UPDATE 5 (s1.output_time <= t + 1) s1.U0LSR);
-       input_list  := TL s1.input_list;  
-       input_time  := t + 5;         
-       output_list := s1.output_list;  
+       input_list  := TL s1.input_list;
+       input_time  := t + 5;
+       output_list := s1.output_list;
        output_time := s1.output_time |>``
   THEN SRW_TAC [] [UART0_READ_def,APPLY_BIT_UPDATE_THM]
   THEN FULL_SIMP_TAC std_ss []);
@@ -187,20 +268,21 @@ val UART0_WRITE = store_thm("UART0_WRITE",
   ``!t s1 w. uart0_ok t s1 /\ s1.U0LSR ' 5 ==>
              ?s2. UART0_NEXT t [MEM_WRITE 0xE000C000w w] s1 s2``,
   SIMP_TAC std_ss [uart0_ok_def,UART0_NEXT_def,MEM,memory_access_11,
-    memory_access_distinct,MEM_WRITE_VALUE_def]
+    memory_access_distinct,BYTE_WRITTEN_TO_MEM_def]
   THEN REPEAT STRIP_TAC
-  THEN EXISTS_TAC 
+  THEN EXISTS_TAC
   ``<| U0RBR := if s1.input_time <= t + 1 /\ s1.input_list <> [] then HD s1.input_list else ARB;
        U0THR := w2w (w:word8);
        U0LCR := s1.U0LCR;
-       U0LSR := BIT_UPDATE 0 (s1.input_time <= t + 1 /\ s1.input_list <> []) 
+       U0LSR := BIT_UPDATE 0 (s1.input_time <= t + 1 /\ s1.input_list <> [])
                (BIT_UPDATE 5 F s1.U0LSR);
-       input_list  := s1.input_list;  
-       input_time  := s1.input_time;         
-       output_list := (w2w (w:word8)) :: s1.output_list;  
+       input_list  := s1.input_list;
+       input_time  := s1.input_time;
+       output_list := (w2w (w:word8)) :: s1.output_list;
        output_time := t + 5 |>``
   THEN SRW_TAC [] [UART0_READ_def,APPLY_BIT_UPDATE_THM]
   THEN FULL_SIMP_TAC std_ss []);
-  
+
+*)
 
 val _ = export_theory();
